\documentclass[10pt,a4paper]{article}
\usepackage[utf8]{inputenc}
\usepackage{amsmath, amsfonts, amssymb, amsthm}
\usepackage{mathtools, array, enumitem, xcolor}
\usepackage[margin=0.7in]{geometry}
\setlength{\parindent}{0em}

\usepackage[czech]{babel}

\theoremstyle{plain}
\newtheorem{veta}{Věta}
\theoremstyle{definition}
\newtheorem{definice}[veta]{Definice}


\title{Řešení domácího úkolu z MA č. 6}
\author{přezdívka: Zdeněk}
\date{}

\begin{document}

\maketitle

\begin{enumerate}

\item 
\[ 
\lim_{x \to -8} \frac{\sqrt{1-x}-3}{2+\sqrt[3]{x}} 
=\lim_{x \to 0} \frac{\sqrt{9-x}-3}{2+\sqrt[3]{x-8}}
=\lim_{x \to 0} \frac{9-x-9}{(2+\sqrt[3]{x-8})(\sqrt{9-x}+3)}
\]\[
=\lim_{x \to 0} -\frac{x(4-2\sqrt[3]{x-8} +(\sqrt[3]{x-8})^2)}{(8+x-8)(\sqrt{9-x}+3)}
\]\[
=\lim_{x \to 0} -\frac{4-2\sqrt[3]{x-8} +(\sqrt[3]{x-8})^2}{\sqrt{9-x}+3}
\]\[
= - \frac{(4-2(-2)+ (-2)^2)}{3+3} = -\frac{12}{6} =-2
\]

\item \[\lim_{x \to 1} \left( \frac{m}{1-x^m} -\frac{n}{1-x^n} \right)\]

Bez újmy na obecnosti předpokládejme $m < n$ a nechť $n = m + l$.

\[ \frac{m(1+x+x^2+ ... + x^{n-1}) -  n(1+x+x^2+ ... + x^{m-1})}{(1-x)(1+x^2+ ... + x^{n-1})(1+x+x^2+ ... + x^{m-1})}
\]\[
= \frac{-l -lx -... -lx^{m-1} + mx^m + mx^{m+1} + ... + mx^{m+l-1}}{(1-x)(1+x^2+ ... + x^{m+l-1})(1+x+x^2+ ... + x^{m-1})}
\]\[
= - \frac{mx^{m+l-2} + 2mx^{m+l-3} + ... + lmx^{m-1} }{(1+x^2+ ... + x^{m+l-1})(1+x^2+ ... + x^{m-1})}
 - \frac{l(m-1)x^{m-2} +l(m-2)x^{m-3} + ... + l  }{(1+x^2+ ... + x^{m+l-1})(1+x^2+ ... + x^{m-1})} \]

Tedy 
 
 \[ \lim_{x \to 1} \left( \frac{m}{1-x^m} -\frac{n}{1-x^n} \right) 
 = \frac{m(1+2+...+(l-1)) + l(m + (m-1) + ... + 1)}{mn}\]\[ 
 =  - \frac{m\frac{l(l-1)}{2} + \frac{ml(m+1)}{2}}{mn}\]\[
= - \frac{ml(m+l)}{2mn} =  - \frac{m(n-m)(m+n-m)}{2mn} = \frac{m-n}{2}
 \]

\item  \[\lim_{x \to a} \left( \frac{\sin(x)}{\sin(a)}\right)^\frac{1}{x-a}\]

\[ = \lim_{x \to 0} \left( \frac{\sin(x+a)}{\sin(a)}\right)^\frac{1}{x} 
  = \lim_{x \to 0} \left( \frac{\sin(x)\cos(a) + \sin(a)\cos(x)}{\sin(a)}\right)^\frac{1}{x} 
\]\[
=\lim_{x \to 0} \left( \sin(x)\cot(a) + \cos(x)\right)^\frac{1}{x} 
\]
\[
  = \lim_{x \to 0} \left( 1 + (\sin(x)\cot(a) + \cos(x)-1) \right)^{\frac{1}{x} \cdot \frac{\sin(x)\cot(a) + \cos(x)-1}{\sin(x)\cot(a) + \cos(x)-1} }
  = \lim_{x \to 0} \exp\left(\cot(a)\frac{\sin(x)}{x} + \frac{\cos(x)-1}{x}\right)
\]\[ 
 = \lim_{x \to 0} \exp\left(\cot(a) + \frac{\cos(x)^2-1}{x(\cos(x)+1)}\right)
 = \lim_{x \to 0} \exp\left(\cot(a) + \frac{x \sin^2(x)}{2x^2}\right) 
\]  \[
= e^{\cot(a) + \frac02} =e^{\cot(a)}
\]
\end{enumerate}


\end{document}