\documentclass[10pt,a4paper]{article}
\usepackage[utf8]{inputenc}
\usepackage{amsmath, amsfonts, amssymb, amsthm}
\usepackage{mathtools, array, enumitem, xcolor}
\usepackage[margin=0.7in]{geometry}
\setlength{\parindent}{0em}

\usepackage[czech]{babel}

\theoremstyle{plain}
\newtheorem{veta}{Věta}
\theoremstyle{definition}
\newtheorem{definice}[veta]{Definice}



\title{Řešení domácího úkolu z MA č. 7}
\author{přezdívka: Zdeněk}
\date{}

\begin{document}

\maketitle

\section{}

\[ f(x) = \arctan\left(\sqrt{x+5}+ \frac5{\sin(x)}\right) e^{5 ln(x^5 + 1) + x^5} \]

\[ \frac{df}{dx} = \left(\frac{d}{dx} \arctan\left(\sqrt{x+5}+ \frac5{\sin(x)}\right)\right)e^{5 ln(x^5 + 1) + x^5} +  \arctan\left(\sqrt{x+5}+ \frac5{\sin(x)}\right)\left(\frac{d}{dx}e^{5 ln(x^5 + 1) + x^5}\right) \]

\begin{align*}
=\left(\frac{d}{dx} \left(\sqrt{x+5}+ \frac5{\sin(x)}\right)\right)\frac{1}{1+ \left( \sqrt{x+5}+ \frac5{\sin(x)} \right)^2}e^{5 ln(x^5 + 1) + x^5} + \\ \arctan\left(\sqrt{x+5}+ \frac5{\sin(x)}\right)\left(\frac{d}{dx} (5 ln(x^5 + 1) + x^5) \right)e^{5 ln(x^5 + 1) + x^5} 
\end{align*}
\begin{align*}
= \left(\frac1{2\sqrt{x+5}} - \frac{5\cos x}{\sin^2(x)}\right)\frac{1}{1+ \left( \sqrt{x+5}+ \frac5{\sin(x)} \right)^2}e^{5 ln(x^5 + 1) + x^5} + \\ \arctan\left(\sqrt{x+5}+ \frac5{\sin(x)}\right)\left(\frac{25x^4}{x^5+1} + 5x^4 \right)e^{5 ln(x^5 + 1) + x^5}
\end{align*}

\section{}

\begin{enumerate}[label=(\alph*)]
\item \[ \lim_{x \to 0} \frac{a^x + a^{-x} - 2}{x^2} 
\overset{L'H}{=} \lim_{x \to 0} \frac{(a^x - a^{-x})\ln(a)}{2x} 
\overset{L'H}{=} \lim_{x \to 0} \frac{(a^x + a^{-x})\ln^2(a)}{2} = \ln^2(a)
\]
Pro hodnoty a, kde to má smysl.

\item \[ \lim_{x \to 0} \left( \frac1{x^2} - \frac1{\sin^2(x)} \right)
= \lim_{x \to 0}  \frac{\sin^2(x)-x^2}{x^2\sin^2(x)} 
\overset{L'H}{=}  \lim_{x \to 0}  \frac{2\sin(x)\cos(x)-2x}{2x\sin^2(x) + 2x^2\sin(x)\cos(x)} \]\[
\overset{L'H}{=}  \lim_{x \to 0}  \frac{2\cos^2(x)-2\sin^2(x)-2}{2\sin^2(x) + 4x\sin(x)\cos(x) + 4x\sin(x)\cos(x) + 2x^2(\cos^2(x) - \sin^2(x))} 
\]\[
= \lim_{x \to 0}  \frac{\cos^2(x)- \sin^2(x)-1}{\sin^2(x) + 4x\sin(x)\cos(x) + x^2\cos^2(x) - x^2\sin^2(x)} \]

\[
\overset{L'H}{=}  \frac{-2\cos(x)\sin(x) - 2\cos(x)\sin(x)}{
\begin{multlined} 
2\cos(x)\sin(x) + 4 (x \cos^2(x) + \cos(x)\sin(x) - x\sin^2(x)) \\ + 2x \cos(x) (\cos(x) - x\sin(x)) - 2x \sin(x) (\sin(x) + x\cos(x))
\end{multlined}
}
\]
\[
=  \frac{-4\cos(x)\sin(x)}{
\begin{multlined} 
2\cos(x)\sin(x) + 4x\cos^2(x)+ 4\cos(x)\sin(x) +4x\sin^2(x) \\ + 2x \cos^2(x) -  2x^2 \cos(x)\sin(x)  - 2x \sin^2(x) - 2x^2 \sin(x)\cos(x)
\end{multlined}
}
\]
\[
=  \frac{-2\cos(x)\sin(x)}{
\begin{multlined} 
3\cos(x)\sin(x) + 2x\cos^2(x) + x - 2x^2 \cos(x)\sin(x) 
\end{multlined}
}
\]
\[
\overset{L'H}{=}  \frac{-2\cos^2(x) + 2\sin^2(x)}{
\begin{multlined} 
3\cos^2(x) - 3\sin^2(x) + 2\cos^2(x) - 4x\cos(x)sin(x) + 1 -  4x \cos(x)\sin(x)
-2x^2 \cos^2(x) + 2x^2\sin^2(x)
\end{multlined}
}
\]
\[
=  \frac{-2}{3 + 2 + 1} = - \frac13
\]
\end{enumerate}

\end{document}