\documentclass[10pt,a4paper]{article}
\usepackage[utf8]{inputenc}
\usepackage{amsmath, amsfonts, amssymb, amsthm}
\usepackage{mathtools, array, enumitem, xcolor}
\usepackage[margin=0.7in]{geometry}
\setlength{\parindent}{0em}

\usepackage[czech]{babel}

\theoremstyle{plain}
\newtheorem{veta}{Věta}
\theoremstyle{definition}
\newtheorem{definice}[veta]{Definice}


\title{Řešení domácího úkolu z MA č. 11}
\author{přezdívka: Zdeněk}
\date{}

\begin{document}

\maketitle

\section{}

\[ \int x \arctan(x) dx \overset{PP}{=} \frac12 x^2 \arctan(x) - \int \frac{x^2}{2(x^2+1)} dx
=  \frac12 x^2 \arctan(x) - \frac12 \int \frac{x^2 + 1 - 1}{x^2+1} dx \]\[
=  \frac12 x^2 \arctan(x) - \frac12 \left(x -  \int \frac{1}{x^2+1} dx \right)  \]\[
=  \frac12 x^2 \arctan(x) - \frac12 x + \frac12\arctan(x) + C 
\]\[
=  \frac{x^2 + 1}2  \arctan(x) - \frac{x}2  + C 
\]

Zpětná derivace:

\[ \frac{d}{dx} \left( \frac{x^2 + 1}2  \arctan(x) - \frac{x}2  + C  \right)
= \frac1{x^2 + 1}\frac{x^2 + 1}2 + \arctan(x) x  - \frac12 =  \arctan(x) x  \]

\section{}
\[
\int x^3 e^{-x^2} dx 
\]

\[ u = -x^2 \]
\[ \frac{du}{dx} = -2x \implies dx = \frac{du}{-2x} \]

\[ \int -ux e^{u}  \frac{du}{-2x}   = \frac12 \int ue^{u}  du  \]\[
\overset{PP}{=}  \frac12 \left( ue^{u} - \int e^{u}  du \right) =    \frac12 \left( ue^{u} - e^{u} \right) + C  \]
\[ = - \frac{x^2 + 1}{2e^{x^2}}  \]


Zpětná derivace:

\[
 \frac{d}{dx} \left(- \frac{x^2 + 1}{2e^{x^2}} \right)
 = - \frac12 \frac{2xe^{x^2} - (x^2 + 1) 2xe^{x^2}}{e^{2x^2}}
 =  - \frac{x - (x^2 + 1) x}{e^{x^2}}
 = x^3 e^{-x^2}
\]

\section{}

\[ \int \frac{6x^3 + 6}{x^3 - 5x^2 + 6x} dx = 6 \int \frac{x^3 + 1}{x^3 - 5x^2 + 6x} dx  \] 
\[
6 \int 1 + \frac{5x^2 - 6x + 1}{x^3 - 5x^2 + 6x} dx = 6x + 6 \int   \frac{5x^2 - 6x + 1}{x(x-2)(x-3)} dx 
\]

Zlomek rozložíme na parciální zlomky 

\[ \frac{A}{x} + \frac{B}{x-2} + \frac{C}{x-3} \]

Vychází $A = 1$ $B =27$ $C = 2$

\[ \int \frac{6x^3 + 6}{x^3 - 5x^2 + 6x} dx = 6x + \ln(|x|) + 27\ln(|x-2|) + 2\ln(|x-3|) \]


\end{document}